### 公式与证明

#### 公式 $S_k(n)$ 定义

$$
S_k(n) = e^{jk\frac{2\pi}{N}n}
$$

#### 1. 证明 $S_k(n) = S_{k+N}(n)$

$$
\begin{aligned}
S_{k+N}(n) &= e^{j(k+N)\frac{2\pi}{N}n} \\
&= e^{jk\frac{2\pi}{N}n} \cdot e^{jN\frac{2\pi}{N}n} \\
&= e^{jk\frac{2\pi}{N}n} \cdot e^{j2\pi n} \\
&= e^{jk\frac{2\pi}{N}n} \cdot (\cos(2\pi n) + j\sin(2\pi n)) \\
&= e^{jk\frac{2\pi}{N}n} \cdot 1 \\
&= S_k(n)
\end{aligned}
$$

因此，$S_{k+N}(n) = S_k(n)$。

#### 2. 证明 $S_k(n) = S^*_{k-N}(n)$

$$
\begin{aligned}
S^*_{k-N}(n) &= e^{-j(k-N)\frac{2\pi}{N}n} \\
&= e^{j(N-k)\frac{2\pi}{N}n} \\
&= e^{jk\frac{2\pi}{N}n} \cdot e^{-jN\frac{2\pi}{N}n} \\
&= e^{jk\frac{2\pi}{N}n} \cdot e^{-j2\pi n} \\
&= e^{jk\frac{2\pi}{N}n} \cdot (\cos(-2\pi n) + j\sin(-2\pi n)) \\
&= e^{jk\frac{2\pi}{N}n} \cdot 1 \\
&= S_k(n)
\end{aligned}
$$

因此，$S^*_{k-N}(n) = S_k(n)$。